src/Std/Data/TreeSet/RawLemmas.lean
@@ -96,4 +96,59 @@ theorem containsThenInsert_snd [TransCmp cmp] (h : t.WF) {k : α} :
     (t.containsThenInsert k).2 = t.insert k :=
   ext <| TreeMap.Raw.containsThenInsert_snd h
 
+@[simp]
+theorem isEmpty_insertIfNew [TransCmp cmp] (h : t.WF) {k : α} :
+    (t.insertIfNew k).isEmpty = false :=
+  DTreeMap.Raw.isEmpty_insertIfNew h
+
+@[simp]
+theorem contains_insertIfNew [TransCmp cmp] (h : t.WF) {k a : α} :
+    (t.insertIfNew k).contains a = (cmp k a == .eq || t.contains a) :=
+  DTreeMap.Raw.contains_insertIfNew h
+
+@[simp]
+theorem mem_insertIfNew [TransCmp cmp] (h : t.WF) {k a : α} :
+    a ∈ t.insertIfNew k ↔ cmp k a == .eq ∨ a ∈ t :=
+  DTreeMap.Raw.mem_insertIfNew h
+
+theorem contains_insertIfNew_self [TransCmp cmp] (h : t.WF) {k : α} :
+    (t.insertIfNew k).contains k :=
+  DTreeMap.Raw.contains_insertIfNew_self h
+
+theorem mem_insertIfNew_self [TransCmp cmp] (h : t.WF) {k : α} :
+    k ∈ t.insertIfNew k :=
+  DTreeMap.Raw.mem_insertIfNew_self h
+
+theorem contains_of_contains_insertIfNew [TransCmp cmp] (h : t.WF) {k a : α} :
+    (t.insertIfNew k).contains a → (cmp k a == .eq) = false → t.contains a :=
+  DTreeMap.Raw.contains_of_contains_insertIfNew h
+
+theorem mem_of_mem_insertIfNew [TransCmp cmp] (h : t.WF) {k a : α} :
+    a ∈ t.insertIfNew k → (cmp k a == .eq) = false → a ∈ t :=
+  DTreeMap.Raw.contains_of_contains_insertIfNew h
+
+/-- This is a restatement of `contains_of_contains_insertIfNew` that is written to exactly match the proof
+obligation in the statement of `get_insertIfNew`. -/
+theorem contains_of_contains_insertIfNew' [TransCmp cmp] (h : t.WF) {k a : α} :
+    (t.insertIfNew k).contains a → ¬((cmp k a == .eq) ∧ t.contains k = false) → t.contains a :=
+  DTreeMap.Raw.contains_of_contains_insertIfNew' h
+
+/-- This is a restatement of `mem_of_mem_insertIfNew` that is written to exactly match the proof obligation
+in the statement of `get_insertIfNew`. -/
+theorem mem_of_mem_insertIfNew' [TransCmp cmp] (h : t.WF) {k a : α} :
+    a ∈ t.insertIfNew k → ¬((cmp k a == .eq) ∧ ¬k ∈ t) → a ∈ t :=
+  DTreeMap.Raw.mem_of_mem_insertIfNew' h
+
+theorem size_insertIfNew [TransCmp cmp] {k : α} (h : t.WF) :
+    (t.insertIfNew k).size = if k ∈ t then t.size else t.size + 1 :=
+  DTreeMap.Raw.size_insertIfNew h
+
+theorem size_le_size_insertIfNew [TransCmp cmp] (h : t.WF) {k : α} :
+    t.size ≤ (t.insertIfNew k).size :=
+  DTreeMap.Raw.size_le_size_insertIfNew h
+
+theorem size_insertIfNew_le [TransCmp cmp] (h : t.WF) {k : α} :
+    (t.insertIfNew k).size ≤ t.size + 1 :=
+  DTreeMap.Raw.size_insertIfNew_le h
+
 end Std.TreeSet.Raw
